Implement 'Node' as an instance of 'OrderedType'.

src/Node.v
@@ -1,5 +1,6 @@
-Require Import Arith.PeanoNat.
+Require Import OrderedType.
 Require Import Classes.RelationClasses.
+Require Import Arith.PeanoNat.
 
 Definition Name := nat.
 Definition Storage := nat.
@@ -8,148 +9,112 @@ Inductive Node : Set :=
 | file : Name -> Storage -> Node
 | dir : Name -> list Node -> Node.
 
-(*****************)
-(* Node equality *)
-(*****************)
+Module Node_as_OT <: OrderedType.
+  Definition t := Node.
 
-Definition eq_node (x1 x2:Node) : Prop :=
-  match x1, x2 with
-  | dir n1 _, dir n2 _ => n1 = n2
-  | file n1 s1, file n2 s2 => n1 = n2 /\ s1 = s2
-  | _, _ => False
-  end.
+  Definition eq (x1 x2:Node) : Prop :=
+    match x1, x2 with
+    | dir n1 _, dir n2 _ => n1 = n2
+    | file n1 s1, file n2 s2 => n1 = n2 /\ s1 = s2
+    | _, _ => False
+    end.
 
-Lemma eq_node_refl : Reflexive eq_node.
-Proof.
-  hnf. destruct x; split; reflexivity.
-Qed.
+  Definition lt (x1 x2:Node) : Prop :=
+    match x1, x2 with
+    | dir n1 _, dir n2 _ => n1 < n2
+    | dir n1 _, file n2 _ => n1 < n2
+    | file n1 _, dir n2 _ => n1 <= n2
+    | file n1 s1, file n2 s2 => (n1 < n2) \/ (n1 = n2 /\ s1 < s2)
+    end.
 
-Lemma eq_node_sym : Symmetric eq_node.
-Proof.
-  hnf. intros. destruct x, y; inversion H.
-  - rewrite H0, H1. split; reflexivity.
-  - reflexivity.
-Qed.
+  Lemma eq_refl : Reflexive eq.
+  Proof.
+    hnf. destruct x; split; reflexivity.
+  Qed.
 
-Lemma eq_node_trans : Transitive eq_node.
-Proof.
-  hnf. intros. destruct x, y, z; inversion H; inversion H0.
-  - rewrite H1, H2, <- H3, <- H4. apply eq_node_refl.
-  - reflexivity.
-Qed.
+  Lemma eq_sym : Symmetric eq.
+  Proof.
+    hnf. intros. destruct x, y; inversion H.
+    - rewrite H0, H1. split; reflexivity.
+    - reflexivity.
+  Qed.
 
-Instance eq_node_equiv : Equivalence eq_node.
-Proof.
-  constructor; [apply eq_node_refl | apply eq_node_sym | apply eq_node_trans].
-Qed.
+  Lemma eq_trans : Transitive eq.
+  Proof.
+    hnf. intros. destruct x, y, z; inversion H; inversion H0.
+    - rewrite H1, H2, <- H3, <- H4. apply eq_refl.
+    - reflexivity.
+  Qed.
 
-(*******************)
-(* Node comparison *)
-(*******************)
-
-Definition compare_node (x1 x2:Node) : comparison :=
-  match x1, x2 with
-  | dir n1 _, dir n2 _ => n1 ?= n2
-  | dir n1 _, file n2 _ => let cmp := n1 ?= n2
-                           in match cmp with
-                              | Eq => Gt
-                              | _ => cmp
-                              end
-  | file n1 _, dir n2 _ => let cmp := n1 ?= n2
-                           in match cmp with
-                              | Eq => Lt
-                              | _ => cmp
-                              end
-  | file n1 s1, file n2 s2 => let cmp := n1 ?= n2
-                              in match cmp with
-                                 | Eq => s1 ?= s2
-                                 | _ => cmp
-                                 end
-  end.
-
-Lemma compare_node_sym :
-  forall (x y:Node), compare_node y x = CompOpp (compare_node x y).
-Proof.
-  intros. destruct x, y; simpl; case_eq (n ?= n0); intro;
-            rewrite Nat.compare_antisym; rewrite H; simpl;
-              reflexivity || apply Nat.compare_antisym.
-Qed.
-
-Lemma compare_node_Eq :
-  forall (x y:Node), compare_node x y = Eq <-> eq_node x y.
-Proof.
-  destruct x, y; simpl; case_eq (n ?= n0); intro.
-  all: match goal with
-       | |- _ <-> False =>
-         split; intro; inversion H0
-       | H : _ = Eq |- _ =>
-         rewrite Nat.compare_eq_iff in H
-       | _ =>
-         split; intro; inversion H0; rewrite <- Nat.compare_eq_iff in H1;
-           rewrite H1 in H; inversion H
+  Ltac destruct_eq :=
+    let Heq := fresh
+    in match goal with
+       | H : ?n = ?n0 /\ _ |- _ =>
+         destruct H as [Heq *]; rewrite Heq || rewrite <- Heq; clear Heq
        end.
-  - rewrite Nat.compare_eq_iff. split; intro; [split | inversion H0]; assumption.
-  - split; intro; [assumption | reflexivity].
-Qed.
 
-Lemma compare_node_Eq_trans : forall (x y z:Node),
-    compare_node x y = Eq -> compare_node y z = Eq -> compare_node x z = Eq.
-Proof.
-  intros. apply compare_node_Eq. apply compare_node_Eq in H.
-  apply compare_node_Eq in H0. transitivity y; assumption.
-Qed.
+  Ltac simpl_cases :=
+    intros; simpl in *;
+    repeat match goal with
+           | H : _ \/ _ |- _ => destruct H
+           end;
+    repeat destruct_eq;
+    match goal with
+    | H : ?n < ?n0, H0 : ?n0 < ?n1 |- _ =>
+      assert (n < n1); [revert H H0; apply Nat.lt_trans|]; clear H H0
+    | H : ?n < ?n0, H0 : ?n0 <= ?n1 |- _ =>
+      assert (n < n1); [revert H H0; apply Nat.lt_le_trans|]; clear H H0
+    | H : ?n <= ?n0, H0 : ?n0 < ?n1 |- _ =>
+      assert (n < n1); [revert H H0; apply Nat.le_lt_trans|]; clear H H0
+    | _ => idtac
+    end.
 
-Ltac destruct_compare_node :=
-  let Hc := fresh
-  in match goal with
-     | H : context [match (?n ?= ?n0) with _ => _ end] |- _ =>
-       case_eq (n ?= n0); intro Hc; rewrite Hc in H; inversion H; clear H
-     end.
+  Lemma lt_trans : forall (x y z:Node), lt x y -> lt y z -> lt x z.
+  Proof.
+    intros. destruct x, y, z; simpl; case_eq (Nat.lt_ge_cases n n1); simpl_cases.
+    all: try assumption || (left; assumption) ||
+             (right; split; [reflexivity | assumption]).
+    all: apply Nat.lt_le_incl; assumption.
+  Qed.
 
-Ltac contradict_compare_node :=
-  let Hn := fresh
-  in simpl in *; repeat destruct_compare_node;
-     repeat match goal with
-            | H : (_ ?= _) = Eq |- _ =>
-              rewrite Nat.compare_eq_iff in H; try rewrite H in *; clear H
-            | H : (_ ?= _) = Lt |- _ =>
-              try rewrite H in *; rewrite Nat.compare_lt_iff in H
-            | H : (_ ?= _) = Gt |- _ =>
-              try rewrite H in *; rewrite Nat.compare_gt_iff in H
-            end;
-     try discriminate;
-     match goal with
-     | H : ?n < ?n0, H0: ?n0 < ?n1 |- _ =>
-       assert (Hn: n < n1); [ revert H H0; apply Nat.lt_trans |]
-     | _ => idtac
-     end;
-     match goal with
-     | H : ?n < ?n |- _ => contradiction (Nat.lt_irrefl n)
-     | H : ?n < ?n0, H0 : ?n0 < ?n |- _ => contradiction (Nat.lt_asymm n n0)
-     | _ => idtac
-     end.
+  Lemma lt_not_eq : forall (x y:Node), lt x y -> ~ eq x y.
+  Proof.
+    intros. unfold not. destruct x, y; simpl in *; try trivial.
+    - intro. destruct H; destruct H0.
+      + rewrite H0 in H. contradiction (Nat.lt_irrefl n0).
+      + destruct H. rewrite H1 in H2. contradiction (Nat.lt_irrefl s0).
+    - intro. rewrite H0 in H. contradiction (Nat.lt_irrefl n0).
+  Qed.
 
-Lemma compare_node_Lt_trans : forall (x y z:Node),
-    compare_node x y = Lt -> compare_node y z = Lt -> compare_node x z = Lt.
-Proof.
-  intros. destruct x, y, z; simpl; case_eq (n ?= n1); intro; try reflexivity;
-            contradict_compare_node. rewrite Nat.compare_lt_iff. assumption.
-Qed.
+  Ltac simpl_compare :=
+    match goal with
+    | H : (_ ?= _) = Eq |- _ =>
+      rewrite Nat.compare_eq_iff in H; rewrite H; clear H
+    | H : (_ ?= _) = Lt |- _ => rewrite Nat.compare_lt_iff in H; apply LT; simpl
+    | H : (_ ?= _) = Gt |- _ => rewrite Nat.compare_gt_iff in H; apply GT; simpl
+    end;
+    try assumption || (left; assumption) || (apply Nat.lt_le_incl; assumption).
 
-Lemma compare_node_Gt_trans : forall (x y z:Node),
-    compare_node x y = Gt -> compare_node y z = Gt -> compare_node x z = Gt.
-Proof.
-  intros. apply (f_equal CompOpp) in H. apply (f_equal CompOpp) in H0.
-  rewrite <- compare_node_sym in H, H0. simpl in H, H0.
-  pose proof (compare_node_Lt_trans z y x H0 H). apply (f_equal CompOpp) in H1.
-  rewrite <- compare_node_sym in H1. assumption.
-Qed.
+  Definition compare : forall (x y:Node), Compare lt eq x y.
+  Proof.
+    intros; destruct x, y; case_eq (n ?= n0); intro; simpl_compare.
+    - case_eq (s ?= s0); intro.
+      + apply Nat.compare_eq_iff in H. rewrite H. apply EQ. split; reflexivity.
+      + apply Nat.compare_lt_iff in H. apply LT.
+        right. split; [reflexivity | assumption].
+      + apply Nat.compare_gt_iff in H. apply GT.
+        right. split; [reflexivity | assumption].
+    - apply LT. simpl. reflexivity.
+    - apply GT. simpl. reflexivity.
+    - apply EQ. simpl. reflexivity.
+  Qed.
 
-Lemma compare_node_trans : forall (c:comparison) (x y z:Node),
-    compare_node x y = c -> compare_node y z = c -> compare_node x z = c.
-Proof.
-  destruct c.
-  - apply compare_node_Eq_trans.
-  - apply compare_node_Lt_trans.
-  - apply compare_node_Gt_trans.
-Qed.
+  Definition eq_dec : forall (x y:Node), {eq x y} + {~ eq x y}.
+  Proof.
+    intros. destruct x, y; simpl; try auto.
+    - case_eq (Nat.eq_dec n n0); case_eq (Nat.eq_dec s s0); intros;
+        try (left; split; assumption) ||
+            (right; unfold not; intro; destruct H1; contradiction).
+    - apply Nat.eq_dec.
+  Qed.
+End Node_as_OT.
